src/kemedhoc/Spec.KEMEDHOC.Ciphertext.fst
@@ -8,18 +8,18 @@ open Spec.KEMEDHOC.KeySchedule
 
 let encrypt_plaintext1 #kcs ptx1 th1 prk1e
   = // derive K1
-  let k1 = expand_k1 #kcs prk1e th1 in
+  let k1 = expand_k #kcs info_label_k1 prk1e th1 in
   // derive IV1
-  let iv1 = expand_iv1 #kcs prk1e th1 in
+  let iv1 = expand_iv #kcs info_label_iv1 prk1e th1 in
   // set up AEAD encryption params
   let ptx1_byte = concat_ptx1 ptx1 in
   aead_encrypt kcs k1 iv1 th1 ptx1_byte
 
 let decrypt_ciphertext1 #kcs ciphertext1 th1 prk1e
   = // derive K1
-  let k1 = expand_k1 #kcs prk1e th1 in
+  let k1 = expand_k #kcs info_label_k1 prk1e th1 in
   // derive IV1
-  let iv1 = expand_iv1 #kcs prk1e th1 in
+  let iv1 = expand_iv #kcs info_label_iv1 prk1e th1 in
   aead_decrypt kcs k1 iv1 th1 ciphertext1
 
 let lemma_encrypt_decrypt_p1_correctness #kcs ptx1 th1 prk1e
@@ -31,17 +31,17 @@ let lemma_encrypt_decrypt_p1_correctness #kcs ptx1 th1 prk1e
 
 let encrypt_plaintext2 #kcs ptx2 th2 prk2e
   = // derive K2
-  let k2 = expand_k2 #kcs prk2e th2 in
+  let k2 = expand_k #kcs info_label_k2 prk2e th2 in
   // derive IV2
-  let iv2 = expand_iv2 #kcs prk2e th2 in
+  let iv2 = expand_iv #kcs info_label_iv2 prk2e th2 in
   let ptx2_byte = concat_ptx2 ptx2 in
   aead_encrypt kcs k2 iv2 th2 ptx2_byte
 
 let decrypt_ciphertext2 #kcs ciphertext2 th2 prk2e
   = // derive K2
-  let k2 = expand_k2 #kcs prk2e th2 in
+  let k2 = expand_k #kcs info_label_k2 prk2e th2 in
   // derive IV2
-  let iv2 = expand_iv2 #kcs prk2e th2 in
+  let iv2 = expand_iv #kcs info_label_iv2 prk2e th2 in
   aead_decrypt kcs k2 iv2 th2 ciphertext2
 
 let lemma_encrypt_decrypt_p2_correctness #kcs ptx2 th2 prk2e
@@ -53,17 +53,17 @@ let lemma_encrypt_decrypt_p2_correctness #kcs ptx2 th2 prk2e
 
 let encrypt_plaintext3 #kcs ptx3 th3 prk3e2m
   = // derive K3
-  let k3 = expand_k3 #kcs prk3e2m th3 in
+  let k3 = expand_k #kcs info_label_k3 prk3e2m th3 in
   // derive IV3
-  let iv3 = expand_iv3 #kcs prk3e2m th3 in
+  let iv3 = expand_iv #kcs info_label_iv3 prk3e2m th3 in
   let ptx3_byte = concat_ptx3 ptx3 in
   aead_encrypt kcs k3 iv3 th3 ptx3_byte
 
 let decrypt_ciphertext3 #kcs ciphertext3 th3 prk3e2m
   = // derive K3
-  let k3 = expand_k3 #kcs prk3e2m th3 in
+  let k3 = expand_k #kcs info_label_k3 prk3e2m th3 in
   // derive IV3
-  let iv3 = expand_iv3 #kcs prk3e2m th3 in
+  let iv3 = expand_iv #kcs info_label_iv3 prk3e2m th3 in
   aead_decrypt kcs k3 iv3 th3 ciphertext3
 
 let lemma_encrypt_decrypt_p3_correctness #kcs ptx3 th3 prk3e2m
